![[Pasted image 20230507142639.png]]
## Theorems:
![[Pasted image 20230507142817.png]]
1. $A'(x) = f(x)$
- $\Longrightarrow A(x) = \int f(x)$
2. If $F'(x) = f(x)$
- $\Longrightarrow \int f(x) dx = F(x)+C$
- $\Longrightarrow \int_a^b f(x)dx = F(b)-F(a)$ 

### Properties
1. $\int_a^b f(x)dx = \int_a^b f(y)dx = \int_a^b f(z)dx$
2. $\int_a^b f(x)dx = -\int_b^a f(x)dx$
3. $\int_a^c f(x)dx = \int_a^b f(x)dx + \int_b^c f(x)dx$
4. 
5. $\int_a^b f(x)dx = \int_a^b f(a+b-x)dx$   (King Rule)  (after appliying king rule add the result with the main eqution)   #imp
6. $\int_0^{2a} f(x)dx = \int_0^a f(x)dx + \int_0^2 f(2a-x)dx$

- $\int_0^{\frac \pi 2} \frac{sin^nx}{cos^nx + sin^nx}dx = \int_0^{\frac \pi 2} \frac{cos^nx}{cos^nx + sin^nx}dx = \frac \pi 4$


